@prefix aio: <https://paul.ti.rw.fau.de/~jo00defe/SemWoT/aio#> .
@prefix rdf: <http://www.w3.org/1999/02/22-rdf-syntax-ns#> .
@prefix owl: <http://www.w3.org/2002/07/owl#> .
@prefix dcterms: <http://purl.org/dc/terms#> .
@prefix dct: <http://purl.org/dc/terms#> .
@prefix vann: <http://vocab.org/vann#> .
@prefix rdfs: <http://www.w3.org/2000/01/rdf-schema#> .
@prefix xsd: <http://www.w3.org/2001/XMLSchema#> .

aio: rdf:type owl:Ontology ;
    dcterms:title "Actionable IoT Ontology" ;
    dcterms:creator "Peter Schiller" , "Michael Freund" ;
    dcterms:description """
    The Actionable IoT Ontology (AIO) captures the interaction patterns and functionalities within the Internet of Things (IoT) domain. 
    It defines key classes to represent interactions with IoT devices, focusing on the "status" field that reflects the current state after an interaction.
    """ ;
    vann:preferredNamespacePrefix "aio" ;
    owl:versionInfo "0.1" .

aio:InteractionInvocation rdf:type rdfs:Class ;
    rdfs:label "Interaction Invocation" ;
    rdfs:comment "Used to describe an interaction with a Thing." .

aio:status rdf:type rdf:Property ;
    rdfs:label "hasStatus" ;
    rdfs:comment "Returns the current status of the Thing that was executed by the action." ;
    rdfs:domain aio:InteractionInvocation ;
    rdfs:range xsd:string .

aio:resultTime rdf:type rdf:Property ;
    rdfs:label "hasResultTime" ;
    rdfs:comment "Returns the time of access." ;
    rdfs:domain aio:InteractionInvocation ;
    rdfs:range xsd:dateTimeStamp .

aio:WritePropertyInteraction rdf:type rdfs:Class ;
    rdfs:label "Write Property" ;
    rdfs:comment "Allows the use of the write property functionality by providing a value." ;
    rdfs:subClassOf aio:InteractionInvocation .

aio:ActionInvocationInteraction rdf:type rdfs:Class ;
    rdfs:label "Action Invocation" ;
    rdfs:comment "An action that allows invoking a function of the Thing, which manipulates states or triggers a process on the Thing." ;
    rdfs:subClassOf aio:InteractionInvocation .

aio:EventSubscriptionInteraction rdf:type rdfs:Class ;
    rdfs:label "Event Subscription" ;
    rdfs:comment "Responsible for subscribing to events from a Thing, implemented using short polling." ;
    rdfs:subClassOf aio:InteractionInvocation .

aio:InvocationInput rdf:type rdfs:Class ;
    rdfs:label "Invocation Input" ;
    rdfs:comment "Describes the input of an invocation such as datatype or numerical value" .

aio:InvocationOutput rdf:type rdfs:Class ;
    rdfs:label "Invocation Output" ;
    rdfs:comment "Describes the output of an invocation such as datatype or numerical value" .

aio:hasInvocationInput rdf:type rdf:Property ;
    rdfs:label "hasInvocationInput" ;
    rdfs:comment "Aligns an interaction invocation with its input information." ;
    rdfs:domain aio:InteractionInvocation ;
    rdfs:range aio:InvocationInput .

aio:hasInvocationOutput rdf:type rdf:Property ;
    rdfs:label "hasInvocationOutput" ;
    rdfs:comment "Aligns an interaction invocation with its output information." ;
    rdfs:domain aio:InteractionInvocation ;
    rdfs:range aio:InvocationOutput .